# Homework

## 9.2

(a) $R_{ijk}^l=L_{ik}{L^l}_j-L_{ij}{L^l}_k=-(L_{ij}{L^l}_k-L_{ik}{L^l}_j)=-R_{ikj}^l$

(b) $R_{ijk}^l+R_{jki}^l+R_{kij}^l
=(L_{ik}L_j^l-L_{ij}L_k^l)+(L_{ji}L_k^l-L_{jk}L_i^l)+(L_{kj}L_i^l-L_{ki}L_j^l)$

$=(L_{ik}L_j^l-L_{ki}L_j^l)+(L_{ji}L_k^l-L_{ij}L_k^l)+(L_{kj}L_i^l-L_{jk}L_i^l)=0$

(c) $\displaystyle
R_{imjk}
=\sum_l R_{ijk}^lg_{lm}
$

$\displaystyle
=\sum_l (L_{ik}{L^l}_j-L_{ij}{L^l}_k)g_{lm}
$

$\displaystyle
=\sum_l (\sum_n({L^n}_kg_{ni}){L^l}_j-\sum_n({L^n}_jg_{ni}){L^l}_k)g_{lm}$

$\displaystyle
=\sum_l\sum_n({L^n}_kg_{ni}L_j^l-{L^n}_jg_{ni}L_k^l)g_{lm}
$

$\displaystyle
=\sum_n\sum_l({L^n}_kg_{lm}L_j^l-{L^n}_jg_{lm}L_k^l)g_{ni}
$

$\displaystyle
=\sum_n\sum_l({L^l}_jg_{lm}{L^n}_k-L_k^lg_{lm}{L^n}_j)g_{ni}
$

$\displaystyle
=-\sum_n\sum_l(L_k^lg_{lm}{L^n}_j-{L^l}_jg_{lm}{L^n}_k)g_{ni}
$

$\displaystyle
=-\sum_n(\sum_l(L_k^lg_{lm}){L^n}_j-\sum_l({L^l}_jg_{lm}){L^n}_k)g_{ni}$

$\displaystyle
=-\sum_n(L_{mk}{L^n}_j-L_{mj}{L^n}_k)g_{ni}$

$\displaystyle
=-\sum_n R_{mjk}^ng_{ni}
=-R_{mijk}$

(d) $\displaystyle
R_{imjk}
=\sum_l R_{ijk}^lg_{lm}$

$\displaystyle
=\sum_l (L_{ik}{L^l}_j-L_{ij}{L^l}_k)g_{lm} 
$

$\displaystyle
=\sum_l (L_{ik}\sum_n(L_{nj}g^{nl})-L_{ij}\sum_n(L_{nk}g^{nl}))g_{lm}$

$\displaystyle
=\sum_l\sum_n(L_{ik}L_{nj}-L_{ij}L_{nk})g_{lm}g^{nl}$

$\displaystyle
=\sum_n(L_{ik}L_{nj}-L_{ij}L_{nk})\delta_m^n$

$\displaystyle
=L_{ik}L_{mj}-L_{ij}L_{mk}$

$\displaystyle
=L_{ki}L_{jm}-L_{ji}L_{km}$

$\displaystyle
=L_{jm}L_{ki}-L_{ji}L_{km}$

$R_{jkim}$



## 9.5

## 9.6

## 9.7

## 9.8

## 9.9

## 9.10

## 9.11

## 9.12

